complete proofs of switch lemmas, all cases except OK fixed in asn_strtoimax_lim_correct

src/C_strtoimax/Switch.v
@@ -1,6 +1,6 @@
+Require Import StructTact.StructTactics.
 Require Import Core.Core Core.Tactics Core.PtrLemmas.
 Require Import C_strtoimax.AST C_strtoimax.Spec.
-Require Import StructTact.StructTactics.
 
 Import ListNotations.
 
@@ -10,31 +10,25 @@ Local Open Scope Int64Scope.
 
 Definition switch :=
 (Sswitch (Ederef (Etempvar _str (tptr tschar)) tschar)
-           (LScons (Some 45)
+       (LScons (Some 45)
+          (Ssequence
+             (Sset _last_digit_max
+                (Ebinop Oadd (Etempvar _last_digit_max tlong) (Econst_int (Int.repr 1) tint)
+                   tlong)) (Sset _sign (Eunop Oneg (Econst_int (Int.repr 1) tint) tint)))
+          (LScons (Some 43)
              (Ssequence
-               (Sset _last_digit_max
-                 (Ebinop Oadd (Etempvar _last_digit_max tlong)
-                   (Econst_int (Int.repr 1) tint) tlong))
-               (Sset _sign
-                 (Eunop Oneg (Econst_int (Int.repr 1) tint) tint)))
-             (LScons (Some 43)
-               (Ssequence
-                 (Sset _str
-                   (Ebinop Oadd (Etempvar _str (tptr tschar))
-                     (Econst_int (Int.repr 1) tint) (tptr tschar)))
-                 (Ssequence
-                   (Sset _t'5
-                     (Ederef (Etempvar _end (tptr (tptr tschar)))
-                       (tptr tschar)))
-                   (Sifthenelse (Ebinop Oge (Etempvar _str (tptr tschar))
-                                  (Etempvar _t'5 (tptr tschar)) tint)
-                     (Ssequence
-                       (Sassign
-                         (Ederef (Etempvar _end (tptr (tptr tschar)))
-                           (tptr tschar)) (Etempvar _str (tptr tschar)))
-                       (Sreturn (Some (Econst_int (Int.repr (-1)) tint))))
-                     Sskip)))
-               LSnil))).
+                (Sset _str
+                   (Ebinop Oadd (Etempvar _str (tptr tschar)) (Econst_int (Int.repr 1) tint)
+                      (tptr tschar)))
+                (Ssequence
+                   (Sset _t'11 (Ederef (Etempvar _end (tptr (tptr tschar))) (tptr tschar)))
+                   (Sifthenelse
+                      (Ebinop Oge (Etempvar _str (tptr tschar)) (Etempvar _t'11 (tptr tschar))
+                         tint)
+                      (Ssequence
+                         (Sassign (Ederef (Etempvar _end (tptr (tptr tschar))) (tptr tschar))
+                            (Etempvar _str (tptr tschar)))
+                         (Sreturn (Some (Econst_int (Int.repr (-1)) tint)))) Sskip))) LSnil))).
 
 Lemma switch_default_correct : forall m ge e i le b ofs,
     Mem.loadv Mint8signed m (Vptr b ofs) = Some (Vint i) ->
@@ -59,9 +53,9 @@ Proof.
   all: try congruence.
   econstructor.
   all: cbn;  try lia.
-Qed.     
-
-       Lemma exec_loop_minus : forall m ge e le b ofs str_b str_ofs fin_b fin_ofs
+       Qed.
+       
+Lemma exec_loop_minus : forall m ge e le b ofs str_b str_ofs fin_b fin_ofs
                                     intp_b intp_ofs i out s1 s2,
   le!_str = Some (Vptr str_b str_ofs)  ->
   le!_end = Some (Vptr fin_b fin_ofs) ->
@@ -92,7 +86,8 @@ Qed.
 Proof.
 Admitted.
 
-Lemma exec_loop_plus : forall m ge e le b ofs str_b str_ofs fin_b fin_ofs intp_b intp_ofs i out s1 s2,
+Lemma exec_loop_plus : forall m ge e le b ofs str_b str_ofs fin_b fin_ofs
+                              intp_b intp_ofs i out s1 s2,
   le!_str = Some (Vptr str_b str_ofs)  ->
   le!_end = Some (Vptr fin_b fin_ofs) ->
   le!_intp = Some (Vptr intp_b intp_ofs)  ->
@@ -115,47 +110,199 @@ Lemma exec_loop_plus : forall m ge e le b ofs str_b str_ofs fin_b fin_ofs intp_b
                             _last_digit_max <~ Vlong last_digit_max ;
                             _upper_boundary <~ Vlong upper_boundary ; 
                             _sign <~ Vint (Int.repr 1)])
-                            (*(_value <~ Vlong 0%int64)
-                               ((_t'5 <~ Vptr b ofs)
-                                  ((_str <~ Vptr str_b (str_ofs + 1)%ptrofs)
-                                     ((_t'4 <~ Vint plus_char)
-                                        ((_t'6 <~ Vptr b ofs)
-                                           ((_last_digit_max <~ Vlong last_digit_max)
-                                              ((_upper_boundary <~ Vlong upper_boundary)
-                                                 ((_sign <~ Vint (Int.repr 1)) le)))))))*)
                             m s1 t le' m' (Out_return out)) ->
         exists t le', exec_stmt ge e le m (pre_loop s1 s2) t le' m' (Out_return out).
 Admitted.
 
-Lemma exec_loop_none : forall m ge e le b ofs str_b str_ofs fin_b fin_ofs intp_b intp_ofs i out s1 s2,
-  le!_str = Some (Vptr str_b str_ofs)  ->
-  le!_end = Some (Vptr fin_b fin_ofs) ->
-  le!_intp = Some (Vptr intp_b intp_ofs)  ->
-  le ! _upper_boundary = Some (Vlong upper_boundary) ->
-  le ! _sign = Some (Vint (Int.repr 1)) ->
 
-  load_addr Mptr m (fin_b, fin_ofs) = Some (Vptr b ofs) ->
-  addr_ge m (str_b, str_ofs) (b, ofs) = Some false ->
-  load_addr Mint8signed m (str_b, str_ofs) = Some (Vint i) ->
+Lemma exec_loop_none : forall m ge e le b ofs str_b str_ofs fin_b fin_ofs
+                              intp_b intp_ofs i out s1 s2,
+    le!_str = Some (Vptr str_b str_ofs)  ->
+    le!_end = Some (Vptr fin_b fin_ofs) ->
+    le!_intp = Some (Vptr intp_b intp_ofs)  ->
+    le ! _upper_boundary = Some (Vlong upper_boundary) ->
+    le ! _sign = Some (Vint (Int.repr 1)) ->
+    
+    load_addr Mptr m (fin_b, fin_ofs) = Some (Vptr b ofs) ->
+    addr_ge m (str_b, str_ofs) (b, ofs) = Some false ->
+    load_addr Mint8signed m (str_b, str_ofs) = Some (Vint i) ->
+    
+    (i == plus_char)%int = false ->
+    (i == minus_char)%int = false ->
+    
+    forall m', (exists t le', exec_stmt ge e
+      (PTree.set _value (Vlong (cast_int_long Signed (Int.repr 0)))
+       (PTree.set _t'10 (Vint i)
+          (PTree.set _t'12 (Vptr b ofs)
+             (PTree.set _last_digit_max (Vlong last_digit_max)
+                (PTree.set _upper_boundary
+                   (Vlong
+                      ((Int64.not (cast_int_long Signed (Int.repr 0)) >>
+                        Int64.repr (Int.unsigned (Int.repr 1))) //
+                       cast_int_long Signed (Int.repr 10)))
+                   (PTree.set _asn1_intmax_max
+                      (Vlong
+                         (Int64.not (cast_int_long Signed (Int.repr 0)) >>
+                          Int64.repr (Int.unsigned (Int.repr 1))))
+                      (PTree.set _sign (Vint (Int.repr 1)) le)))))))
+                          m s1 t le' m' (Out_return out)) ->
+                   
+     exists t le', exec_stmt ge e le m (pre_loop s1 s2) t le' m' (Out_return out).
+Proof.
+  intros until s2.
+  intros Str End Intp UB Sign LA AG LA' CharP CharM  m' S1.
+  destruct S1.
+  unfold pre_loop.
+  edestruct (switch_default_correct m ge e i
+              (PTree.set _t'10 (Vint i)
+       (PTree.set _t'12 (Vptr b ofs)
+          (PTree.set _last_digit_max
+             (Vlong last_digit_max)
+             (PTree.set _upper_boundary
+                (Vlong
+                   ((Int64.not (cast_int_long Signed (Int.repr 0)) >>
+                     Int64.repr (Int.unsigned (Int.repr 1))) //
+                    cast_int_long Signed (Int.repr 10)))
+                (PTree.set _asn1_intmax_max
+                   (Vlong
+                      (Int64.not (cast_int_long Signed (Int.repr 0)) >>
+                       Int64.repr (Int.unsigned (Int.repr 1))))
+                   (PTree.set _sign (Vint (Int.repr 1)) le))))))).
+  all: repeat rewrite set_env_eq_ptree_set in *;
+    repeat (eassumption || env_assumption).
+  destruct H.
+  repeat eexists.
+  econstructor.
+  repeat econstructor.
+  econstructor.
+  repeat econstructor.
+  econstructor.
+  repeat econstructor.
+  repeat (eassumption || env_assumption).
+  repeat econstructor.
+  econstructor.
+  econstructor.
+  repeat econstructor.
+  repeat env_assumption.
+  econstructor.
+  repeat econstructor.
+  econstructor.
+  repeat econstructor.
+  repeat env_assumption.
+  repeat env_assumption.
+  repeat env_assumption.
+  repeat env_assumption.
+  repeat env_assumption.
+  econstructor.
+  unfold load_addr in *.
+  unfold addr_ge in *.
+  eapply (ptr_ge_to_sem_cmp_false _ _ _ _ _ AG).
+  econstructor.
+  econstructor.
+  econstructor.
+  repeat econstructor.
+  repeat env_assumption.
+  repeat env_assumption.
+  eassumption.
+  apply exec_Sseq_2.
+  econstructor.
+  repeat econstructor.
+  eassumption.
+  congruence.
+Qed.
+  
 
-  (i == plus_char)%int = false ->
-  (i == minus_char)%int = false ->
-
-  forall le' m', (exists t, exec_stmt ge e
-                            (in le set [
-                              _value <~ Vlong (cast_int_long Signed (Int.repr 0)) ;
-                              _t'4 <~ Vint i ;
-                              _t'6 <~ Vptr b ofs ;
-                              _last_digit_max <~ Vlong (Int64.modu 
-                                                       (Int64.not (cast_int_long Signed (Int.repr 0)) >> 
-                                                       Int64.repr (Int.unsigned (Int.repr 1))) 
-                                                       (cast_int_long Signed (Int.repr 10))) ;
-                              _upper_boundary <~ Vlong (Int64.divu
-                                                       (Int64.not (cast_int_long Signed (Int.repr 0)) >> 
-                                                       Int64.repr (Int.unsigned (Int.repr 1))) 
-                                                       (cast_int_long Signed (Int.repr 10))) ;
-                              _sign <~ Vint (Int.repr 1) ])
-                            m s1 t le' m' (Out_return out)) ->
-
-        exists t le', exec_stmt ge e le m (pre_loop s1 s2) t le' m' (Out_return out).
-Admitted.
+Lemma exec_loop_none_out_normal : forall m ge e le b ofs str_b str_ofs fin_b fin_ofs
+                              intp_b intp_ofs i out s1 s2,
+    le!_str = Some (Vptr str_b str_ofs)  ->
+    le!_end = Some (Vptr fin_b fin_ofs) ->
+    le!_intp = Some (Vptr intp_b intp_ofs)  ->
+    le ! _upper_boundary = Some (Vlong upper_boundary) ->
+    le ! _sign = Some (Vint (Int.repr 1)) ->
+    
+    load_addr Mptr m (fin_b, fin_ofs) = Some (Vptr b ofs) ->
+    addr_ge m (str_b, str_ofs) (b, ofs) = Some false ->
+    load_addr Mint8signed m (str_b, str_ofs) = Some (Vint i) ->
+    
+    (i == plus_char)%int = false ->
+    (i == minus_char)%int = false ->
+    
+    forall m' le', (exists t, exec_stmt ge e
+                          (PTree.set _value (Vlong (cast_int_long Signed (Int.repr 0)))
+       (PTree.set _t'10 (Vint i)
+          (PTree.set _t'12 (Vptr b ofs)
+             (PTree.set _last_digit_max (Vlong last_digit_max)
+                (PTree.set _upper_boundary
+                   (Vlong
+                      ((Int64.not (cast_int_long Signed (Int.repr 0)) >>
+                        Int64.repr (Int.unsigned (Int.repr 1))) //
+                       cast_int_long Signed (Int.repr 10)))
+                   (PTree.set _asn1_intmax_max
+                      (Vlong
+                         (Int64.not (cast_int_long Signed (Int.repr 0)) >>
+                          Int64.repr (Int.unsigned (Int.repr 1))))
+                      (PTree.set _sign (Vint (Int.repr 1)) le)))))))
+                          m s1 t le' m' Out_normal) ->
+                    (exists t le'', exec_stmt ge e le'
+       
+                                   m' s2 t le'' m' (Out_return out)) ->
+                    
+                   
+          exists t le'', exec_stmt ge e le m (pre_loop s1 s2) t le'' m' (Out_return out).
+Proof.
+  intros until s2.
+  intros Str End Intp UB Sign LA AG LA' CharP CharM m' le' S1 S2.
+  destruct S1.
+  destruct S2.
+  destruct H0.
+  unfold pre_loop.
+  edestruct (switch_default_correct m ge e i
+              (PTree.set _t'10 (Vint i)
+       (PTree.set _t'12 (Vptr b ofs)
+          (PTree.set _last_digit_max
+             (Vlong last_digit_max)
+             (PTree.set _upper_boundary
+                (Vlong
+                   ((Int64.not (cast_int_long Signed (Int.repr 0)) >>
+                     Int64.repr (Int.unsigned (Int.repr 1))) //
+                    cast_int_long Signed (Int.repr 10)))
+                (PTree.set _asn1_intmax_max
+                   (Vlong
+                      (Int64.not (cast_int_long Signed (Int.repr 0)) >>
+                       Int64.repr (Int.unsigned (Int.repr 1))))
+                   (PTree.set _sign (Vint (Int.repr 1)) le))))))).
+  all: repeat rewrite set_env_eq_ptree_set in *;
+    repeat (eassumption || env_assumption).
+  repeat eexists.
+  econstructor.
+  repeat econstructor.
+  econstructor.
+  repeat econstructor.
+  econstructor.
+  repeat econstructor.
+  repeat (eassumption || env_assumption).
+  repeat econstructor.
+  econstructor.
+  econstructor.
+  repeat econstructor.
+  repeat env_assumption.
+  econstructor.
+  repeat econstructor.
+  repeat econstructor.
+  repeat env_assumption.
+  repeat env_assumption.
+  repeat env_assumption.
+  repeat env_assumption.
+  repeat env_assumption.
+  econstructor.
+  unfold load_addr in *.
+  eapply (ptr_ge_to_sem_cmp_false _ _ _ _ _ AG).
+  forward.
+  econstructor.
+  repeat env_assumption.
+  repeat env_assumption.
+  eassumption.
+  eassumption.
+  eassumption.
+  Qed.
+  
